\begin{grammar}
<program> ::= (<function-definition> | <statement>)*
\end{grammar}
\begin{grammar}
<function-definition> ::= `function' `&'?<function-name> `(' (`&'? <var> ( `,' `&'? <var>)* ) | $\epsilon$`)' <block>
\end{grammar}
\begin{grammar}
<statement> ::= `while (' <expr> `)' <statement>
%\alt `foreach (' <expr> `as' <opt-arrow-var> `)' <statement>
\alt `for (' <expr>?`;'<expr>?`;'<expr>? `)' <statement>
\alt `if('<expr>`)' <statement>
\alt `if('<expr>`)' <statement> `else' <statement>
\alt `;'
\alt <expr>`;'
\alt `global' <var> (`,' <var>)*`;'
\alt `return' (<expr>|<rexpr>)?`;'
\alt <block>
\end{grammar}
\begin{grammar}
<expr> ::= <expr> $\oplus$ <expr>
\alt `!' <expr>
\alt `-' <expr>
\alt `(' <expr> `)'
\alt <var-expr>`+ +'
\alt <var-expr>`- -'
\alt `+ +'<var-expr>
\alt `- -'<var-expr>
\alt <var>
\alt <expr> `['<expr> `]'
\alt <function-reference>
\alt <const>
\alt <assignment>
\alt `[' ($\epsilon$ | <array-init-entry> (`,' <array-init-entry>)*) `]'
\alt `array(' ($\epsilon$ | <array-init-entry> (`,' <array-init-entry>)*) `)'
\end{grammar}
\begin{grammar}
<function-reference> ::= <function-name>`(' (<function-arg> (`,' <function-arg>)* | $\epsilon$ ) `)'
\end{grammar}
\begin{grammar}
<function-arg> ::= <expr> 
\alt <rexpr> 
\end{grammar}
\begin{grammar}
<rexpr> ::= <var> 
\alt <function-reference>
\alt <rexpr>`[]'
\alt <rexpr>`[' <expr> `]'
\end{grammar}
\begin{grammar}
<var-expr> ::= <var> 
\alt <rexpr>`[]'
\alt <rexpr>`[' <expr> `]'
\end{grammar}
\begin{grammar}
<array-init-entry> ::= <expr> `=>' <expr> 
\alt <expr>
\end{grammar}
\begin{grammar}
<assignment> ::= <var-expr> `=' <rexpr>`;'
\alt <var-expr> `=' `&'<rexpr>`;'
\end{grammar}
\begin{grammar}
<block> ::= `{' <statement>* `}'
\end{grammar}